some stuff for sets

theories/Sets.v
@@ -3,66 +3,63 @@ From RocqCandy Require Import All.
 Import MapNotations.
 From Stdlib Require Import List String.
 From Stdlib Require Export ListSet.
+From AttestationMaxims Require Import Tactics.
 Local Open Scope map_scope.
 
 Section Sets.
 
   Context (A : Type) `{DK : DecEq A}.
 
-  Definition union {A} `{DecEq A} := set_union dec_eq.
-  Definition add {A} `{HDA : DecEq A} := set_add dec_eq.
-  Definition mem {A} `{HDA : DecEq A} := set_mem dec_eq.
-
   Definition bin_rel := set (A * A).
+  
+  Lemma length_set_add : forall (s : set A) a,
+    List.length (set_add dec_eq a s) =
+      match set_In_dec dec_eq a s with
+      | left _ => List.length s
+      | right _ => S (List.length s)
+      end.
+  Proof.
+    induction s; ff.
+    - edestruct n; ff.
+    - erewrite IHs; ff.
+    - erewrite IHs; ff.
+      edestruct n0; ff.
+  Qed.
 
   Fixpoint all_in_rel (d : bin_rel) : set A :=
     match d with
     | [] => nil
     | (c1, c2) :: rest => 
-      union (c1 :: c2 :: nil) (all_in_rel rest)
+      set_add dec_eq c1 (set_add dec_eq c2 (all_in_rel rest))
     end.
 
   Fixpoint get_all_one_step_reverse (d : bin_rel) (c : A) : set A :=
     match d with
     | [] => nil
     | (c1, c2) :: rest =>
-        if dec_eq c2 c then add c1 (get_all_one_step_reverse rest c)
+        if dec_eq c2 c then set_add dec_eq c1 (get_all_one_step_reverse rest c)
         else get_all_one_step_reverse rest c
     end.
+  
+  Lemma in_get_all_one_step_reverse_impl_in_all_in_rel : forall (d : bin_rel) (c c' : A),
+    In c' (get_all_one_step_reverse d c) ->
+    In c' (all_in_rel d).
+  Proof.
+    induction d; ff.
+    repeat (erewrite set_add_iff in *); ff.
+    eapply IHd in H.
+    repeat (erewrite set_add_iff in *); ff.
+  Qed.
 
   Lemma not_set_In_add : forall {A} `{DecEq A} s (a : A),
     ~ set_In a s ->
-    List.length (add a s) = S (List.length s).
+    List.length (set_add dec_eq a s) = S (List.length s).
   Proof.
     induction s; ff.
     - edestruct H0; ff.
   Qed.
 
-  Equations? get_multi_step_reverse' (c : A) (rel : set (A * A)) (seen : set A) : set A
-      by wf (List.length (all_in_rel rel) - List.length seen) :=
-  get_multi_step_reverse' c rel seen :=
-    match (List.length (all_in_rel rel) - List.length seen) as n return (List.length (all_in_rel rel) - List.length seen = n -> _) with
-    | 0 => fun Hm => nil
-    | S _ =>
-      fun Hm =>
-      match (set_In_dec (DecEq.dec_eq) c seen) with
-      | left _ => nil
-      | right _ =>
-        let parents := get_all_one_step_reverse rel c in
-        set_fold_left 
-          (fun (acc : set A) c' => union acc (get_multi_step_reverse' c' rel (add c seen)))
-          parents
-          parents
-      end
-    end eq_refl.
-  Proof.
-    erewrite not_set_In_add; ff l.
-  Defined.
-
-  Definition get_multi_step_reverse (c : A) (d : bin_rel) : set A :=
-    get_multi_step_reverse' c d nil.
-
-  
+    
   Lemma in_acc_impl_in_set_fold_union : forall {A} `{HD : DecEq A} (f : A -> set A) (lst : list A) (x : A) (acc : set A),
     (In x acc) ->
     In x (fold_left (fun acc a => set_union dec_eq acc (f a)) lst acc).
@@ -73,7 +70,7 @@ Section Sets.
   Qed.
 
   Lemma set_in_fold_left_union : forall (f : A -> set A) (lst : list A) (x : A) (acc : set A),
-    In x (fold_left (fun acc a => set_union dec_eq acc (f a)) lst acc) <->
+    In x (set_fold_left (fun acc a => set_union dec_eq acc (f a)) lst acc) <->
     (* either in acc to start or in f a*)
     (In x acc) \/ (exists a, In a lst /\ set_In x (f a)).
   Proof.
@@ -99,8 +96,57 @@ Section Sets.
           erewrite set_union_iff; ff.
   Qed.
 
+  Equations? get_multi_step_reverse' (c : A) (rel : set (A * A)) (seen : set A) : set A
+      by wf (List.length (all_in_rel rel) - List.length seen) :=
+  get_multi_step_reverse' c rel seen :=
+    match (List.length (all_in_rel rel) - List.length seen) as n return (List.length (all_in_rel rel) - List.length seen = n -> _) with
+    | 0 => fun Hm => nil
+    | S _ =>
+      fun Hm =>
+      match (set_In_dec (DecEq.dec_eq) c seen) with
+      | left _ => nil
+      | right _ =>
+        let parents := get_all_one_step_reverse rel c in
+        set_fold_left 
+          (fun (acc : set A) c' => set_union dec_eq acc (get_multi_step_reverse' c' rel (set_add dec_eq c seen)))
+          parents
+          parents
+      end
+    end eq_refl.
+  Proof.
+    erewrite not_set_In_add; ff l.
+  Defined.
+
+  Definition get_multi_step_reverse (c : A) (d : bin_rel) : set A :=
+    get_multi_step_reverse' c d nil.
+
+  Definition subset {A} `{DecEq A} (s1 s2 : set A) : Prop :=
+    forall x, set_In x s1 -> set_In x s2.
+
+  Theorem seen_set_always_subset : forall n c rel seen,
+    List.length (all_in_rel rel) - List.length seen <= n ->
+    subset seen (all_in_rel rel) ->
+    In c (all_in_rel rel) ->
+    forall x,
+    set_In x (get_multi_step_reverse' c rel seen) ->
+    subset (x :: seen) (all_in_rel rel).
+  Proof.
+    unfold subset.
+    induction n; ff.
+    - ltac1:(simp get_multi_step_reverse' in *); ff l.
+    - ltac1:(simp get_multi_step_reverse' in *); ff l.
+      erewrite set_in_fold_left_union in *; ff l;
+      elim_all_contras; ff l.
+      * eapply in_get_all_one_step_reverse_impl_in_all_in_rel; ff.
+      * destruct (set_In_dec dec_eq x0 seen); ff.
+        eapply IHn in H3; ff l.
+        + erewrite length_set_add; ff l.
+        + erewrite set_add_iff in *; ff.
+        + eapply in_get_all_one_step_reverse_impl_in_all_in_rel; ff.
+  Qed.
+
   Lemma set_In_add_split : forall (c c' : A) s,
-    set_In c (add c' s) -> c = c' \/ set_In c s.
+    set_In c (set_add dec_eq c' s) -> c = c' \/ set_In c s.
   Proof.
     induction s; ff.
     apply IHs in H0; ff.
@@ -116,7 +162,7 @@ Section Sets.
     Datatypes.length s <> 0 ->
     Datatypes.length (set_union dec_eq s s') <> 0.
   Proof.
-    unfold union. induction s; ff.
+    induction s; ff.
     apply empty_set_length_iff in H0.
     assert (In a (set_union dec_eq (a :: s) s')).
     apply set_union_intro; ff.
@@ -137,6 +183,11 @@ Section Sets.
     rewrite <- add_set_len. auto.
   Qed.
 
+  Lemma union_non_empty_len_more_r : forall (s s' : list A),
+    Datatypes.length s' <= Datatypes.length (set_union dec_eq s s').
+  Proof.
+  Admitted.
+
   Lemma union_non_empty : forall (s s' : list A),
     s <> [] ->
     set_union dec_eq s s' <> [].
@@ -155,13 +206,13 @@ Section Sets.
     - ff.
     - intro. destruct a.
       unfold get_multi_step_reverse in *.
-      ltac1:(simp get_multi_step_reverse' in *); ff; unfold set_fold_left in *; unfold union in *; try (erewrite set_in_fold_left_union in *); ff.
-        rewrite Nat.sub_0_r in Heqn. pp (union_non_empty_len [a; c] (all_in_rel E)); ff l.
-        rewrite Nat.sub_0_r in Heqn. pp (union_non_empty_len [a; c] (all_in_rel E)); ff l.
-        rewrite Nat.sub_0_r in Heqn. pp (union_non_empty_len [a; a0] (all_in_rel E)); ff l.
+      ltac1:(simp get_multi_step_reverse' in *); ff; try (erewrite set_in_fold_left_union in *); ff.
+      * erewrite Nat.sub_0_r in *; try (erewrite length_zero_iff_nil in *); ff.
+      * repeat (erewrite length_set_add in *; ff).
+      * repeat (erewrite length_set_add in *; ff).
   Qed.
 
-  Lemma all_in_rel_empty : forall E,
+  (* Lemma all_in_rel_empty : forall E,
     all_in_rel E = nil <-> E = nil.
   Proof.
     induction E; ff.
@@ -173,7 +224,7 @@ Section Sets.
   Proof.
     induction E; ff.
     apply union_non_empty_len in H; ff.
-  Qed.
+  Qed. *)
 
   Lemma in_dep_rel_one_step : forall c c' E,
     In (c, c') E <->
@@ -201,7 +252,7 @@ Section Sets.
       apply in_dep_rel_one_step. apply H in H0; ff.
   Qed. 
 
-  Lemma expand_dep_rel_test : forall n E sn,
+  Lemma expand_dep_rel_test' : forall n E sn,
     List.length (all_in_rel E) - List.length sn <= n ->
     forall c c',
     In c (get_multi_step_reverse' c' E sn) ->
@@ -209,8 +260,64 @@ Section Sets.
     In c (get_multi_step_reverse' c' (a :: E) sn).
   Proof.
     induction n; ff.
-    - ltac1:(simp get_multi_step_reverse' in *); ff.
-      * Search (set_union _ _ _ _).
+    - ltac1:(simp get_multi_step_reverse' in *); ff l.
+    - ltac1:(simp get_multi_step_reverse' in *); ff l;
+      erewrite set_in_fold_left_union in *; ff l.
+      * assert (S n0 <= 0). {
+          erewrite <- Heqn1, <- Heqn0.
+          erewrite Nat.sub_le_mono_r; ff.
+          repeat (erewrite add_set_len; ff).
+        }
+        lia.
+      * elim_all_contras.
+        + left; eapply set_add_intro; ff.
+        + ff.
+          eapply IHn in H1.
+          --  
+            right.
+            exists v.
+            split; ff.
+            eapply set_add_intro; ff.
+          -- erewrite length_set_add; ff.
+            destruct (List.length (all_in_rel E)); ff l.
+      * elim_all_contras.
+        eapply IHn in H1; ff l.
+        erewrite length_set_add; ff.
+        destruct (List.length (all_in_rel E)); ff l.
+  Qed.
+
+  Lemma get_multi_dep_rel_cons_self : forall a a' E s,
+    (forall x, In x s -> In x (all_in_rel E)) ->
+    ~ (In a s) ->
+    In a' (get_multi_step_reverse' a ((a', a) :: E) s).
+  Proof.
+    intros.
+    ltac1:(simp get_multi_step_reverse' in *); ff l.
+    - admit.
+    - erewrite set_in_fold_left_union in *.
+      left.
+      erewrite set_add_iff; ff.
+  Admitted.
+
+  Lemma get_one_get_multi' : forall n c c' E s,
+    List.length (all_in_rel E) - List.length s <= n ->
+    In c' (get_all_one_step_reverse E c) ->
+    ~ In c s ->
+    In c' (get_multi_step_reverse' c E s).
+  Proof.
+    induction n; ff.
+    - ltac1:(simp get_multi_step_reverse' in *); ff l.
+      admit.
+    - ltac1:(simp get_multi_step_reverse' in *); ff l.
+      * repeat (erewrite length_set_add in *; ff).
+    induction E; ff l.
+    - erewrite set_add_iff in *; elim_all_contras; ff l.
+      * eapply
+        eapply expand_dep_rel_test'; ff.
+        eapply IHE; ff.
+      * eapply expand_dep_rel_test'; ff l; eapply IHE.
+    - eapply expand_dep_rel_test'; ff l; eapply IHE.
+  Admitted.
 
   Lemma expand_dep_rel_test : forall E,
     forall c c',
@@ -218,87 +325,9 @@ Section Sets.
     forall a,
     In c (get_multi_step_reverse c' (a :: E)).
   Proof.
-
-    intros; ff.
-    try (unfold get_multi_step_reverse in *; ltac1:(simp get_multi_step_reverse' in * ); ff; unfold set_fold_left in *; unfold union in *; try (erewrite set_in_fold_left_union in * ); ff);
-    try (rewrite Nat.sub_0_r in * ); try (find_eapply_lem_hyp union_non_empty_len; ff);
-    try (find_eapply_lem_hyp all_in_rel_empty_len; ff);
-    try (find_eapply_lem_hyp length_zero_iff_nil; ff).
-    - admit.
-    - admit.
-  Admitted.
-
-  (* maybe try writing a lemma for when only one component is in the seen set *)
-
-
-  Lemma expand_dep_rel : forall E E',
-    (forall x, In x E -> In x E') ->
-    forall c c',
-    In c (get_multi_step_reverse c' E) ->
-    In c (get_multi_step_reverse c' E').
-  Proof.
-    induction E'; ff.
-    try (unfold get_multi_step_reverse in *; ltac1:(simp get_multi_step_reverse' in * ); ff; unfold set_fold_left in *; unfold union in *; try (erewrite set_in_fold_left_union in * ); ff).
-    destruct H0; ff.
-    - apply in_dep_rel_one_step in H0. eapply H. apply H0.
-    - apply in_dep_rel_one_step in H0. eapply H. apply H0.
-    - destruct a. destruct (dec_eq c' a0).
-      + inversion e; ff. destruct (dec_eq c a0); ff.
-        * admit.
-        * admit.
-      + admit.
-      (* try (unfold get_multi_step_reverse in *; ltac1:(simp get_multi_step_reverse' in * ); ff; unfold set_fold_left in *; unfold union in *; try (erewrite set_in_fold_left_union in * ); ff);
-      try (rewrite Nat.sub_0_r in * ); try (find_eapply_lem_hyp union_non_empty_len; ff);
-      try (find_eapply_lem_hyp all_components_empty_len; ff);
-      try (find_eapply_lem_hyp length_zero_iff_nil; ff).
-
-    induction E; ff. inversion H0.
-      try (unfold get_multi_step_reverse in *; ltac1:(simp get_multi_step_reverse' in * ); ff; unfold set_fold_left in *; unfold union in *; try (erewrite set_in_fold_left_union in * ); ff);
-      try (rewrite Nat.sub_0_r in * ); try (find_eapply_lem_hyp union_non_empty_len; ff);
-      try (find_eapply_lem_hyp all_components_empty_len; ff);
-      try (find_eapply_lem_hyp length_zero_iff_nil; ff).
-      + apply IHE; ff.
-        * apply IHE'; ff. admit.
-        * 
-    
-    try (unfold get_multi_step_reverse in *; ltac1:(simp get_multi_step_reverse' in * ); ff; unfold set_fold_left in *; unfold union in *; try (erewrite set_in_fold_left_union in * ); ff);
-      try (rewrite Nat.sub_0_r in * ); try (find_eapply_lem_hyp union_non_empty_len; ff);
-      try (find_eapply_lem_hyp all_components_empty_len; ff);
-      try (find_eapply_lem_hyp length_zero_iff_nil; ff).
-      destruct H0; ff.
-      + apply in_dep_rel_one_step in H0.
-        pp (H _ H0). elim_contras H0; ff.
-      + 
-      destruct E. admit.
-
-
-    *)
-    (* induction E; ff.
-    - unfold get_multi_step_reverse in *; ltac1:(simp get_multi_step_reverse' in * ); ff.
-    - try (unfold get_multi_step_reverse in *; ltac1:(simp get_multi_step_reverse' in * ); ff; unfold set_fold_left in *; unfold union in *; try (erewrite set_in_fold_left_union in * ); ff);
-      try (rewrite Nat.sub_0_r in * ); try (find_eapply_lem_hyp union_non_empty_len; ff);
-      try (find_eapply_lem_hyp all_components_empty_len; ff);
-      try (find_eapply_lem_hyp length_zero_iff_nil; ff).
-      + elim_contras H0; ff. 
-        * left.
-          pp (H _ (or_introl eq_refl)).
-          apply in_dep_rel_one_step; ff.
-        * ltac1:(simp get_multi_step_reverse' in H1); ff. exfalso; ff.
-      + elim_contras H0; ff.
-        * apply set_add_elim in hc; unfold set_In in *; ff.
-          pp (H _ (or_introl eq_refl)).
-          destruct (dec_eq c c0); ff.
-          -- left.
-            apply in_dep_rel_one_step; ff.
-          -- apply in_dep_rel_one_step in H0. right. exists c0; split; ff.
-          left. admit.
-        * admit.
-      + elim_contras H0; ff.
-        * left. admit.
-        * pp (H _ (or_introl eq_refl)); ff. *)
-  
-  Admitted.
-
+    intros.
+    eapply expand_dep_rel_test'; ff.
+  Qed.
 
   Lemma get_one_step_one_step_trans : forall c c' E,
     In c' (get_all_one_step_reverse E c) -> c' <> c ->
@@ -309,30 +338,6 @@ Section Sets.
   Proof.
     induction E; ff.
   Admitted.
-  (* 
-
-    try (unfold get_multi_step_reverse in *; ltac1:(simp get_multi_step_reverse' in * ); ff; unfold set_fold_left in *; unfold union in *; try (erewrite set_in_fold_left_union in * ); ff; try (rewrite Nat.sub_0_r in * ); find_eapply_lem_hyp union_non_empty_len; ff).
-    - pp (IHE H H0 c'' H1 H2).
-      ff.
-      try (unfold get_multi_step_reverse in *; ltac1:(simp get_multi_step_reverse' in * ); ff; unfold set_fold_left in *; unfold union in *; try (erewrite set_in_fold_left_union in * ); ff);
-      try (rewrite Nat.sub_0_r in * ); try (find_eapply_lem_hyp union_non_empty_len; ff).
-      + find_eapply_lem_hyp all_in_rel_empty_len; ff.
-        find_eapply_lem_hyp length_zero_iff_nil; ff.
-      + right. exists c'; split; ff.
-        try (ltac1:(simp get_multi_step_reverse' in * ); ff; unfold set_fold_left in *; unfold union in *; try (erewrite set_in_fold_left_union in * ); ff).
-        assert (Datatypes.length [c0; c'] = 2).
-        * simpl. reflexivity.
-        * assert (2 <= Datatypes.length (set_union dec_eq [c0; c'] (all_in_rel E))). rewrite <- H5. apply union_non_empty_len_more.
-            lia.
-    - destruct (dec_eq c' c0); ff.
-      + admit.
-      + assert (In c' (get_all_one_step_reverse E c)).
-        apply set_add_elim in H. destruct H; ff.
-        pp (IHE H4 H0 c'' H1 H2 H3). admit.
-    - admit.
-  Admitted.
-  *)
-
 
   Lemma get_one_step_multi_step_trans : forall c c' E,
     In c' (get_all_one_step_reverse E c) ->
@@ -341,7 +346,7 @@ Section Sets.
       In c'' (get_multi_step_reverse c E).
   Proof.
     induction E; ff.
-    unfold get_multi_step_reverse in *; ltac1:(simp get_multi_step_reverse' in *); ff; unfold set_fold_left in *; unfold union in *; erewrite set_in_fold_left_union in *.
+    unfold get_multi_step_reverse in *; ltac1:(simp get_multi_step_reverse' in *); ff; erewrite set_in_fold_left_union in *.
     - admit.
     - admit.
   Admitted.
@@ -363,9 +368,8 @@ Section Sets.
     unfold get_multi_step_reverse.
     ltac1:(simp get_multi_step_reverse' in *); ff.
     - rewrite Nat.sub_0_r in Heqn. apply union_non_empty_len in Heqn; ff.
-    - unfold set_fold_left in *; unfold union in *; erewrite set_in_fold_left_union in *.
-      destruct (dec_eq c'' a0); ff.
-    - unfold set_fold_left in *; unfold union in *; erewrite set_in_fold_left_union in *.
+    - erewrite set_in_fold_left_union in *; destruct (dec_eq c'' a0); ff.
+    - erewrite set_in_fold_left_union in *.
       assert (In c' (get_multi_step_reverse c E)) by admit.
       destruct (dec_eq c'' a0).
       + admit.
@@ -378,17 +382,119 @@ Section Sets.
       In c'' (get_multi_step_reverse c E).
   Admitted.
 
-  Lemma get_multi_step_reverse_trans : forall c c' E s,
+  Lemma get_multi_step_self_nil : forall s c c' E,
+    ~ (set_In c' (get_multi_step_reverse' c E (set_add dec_eq c s))).
+  Proof.
+    intros.
+    ltac1:(simp get_multi_step_reverse' in *); ff.
+    eapply n0.
+    erewrite set_add_iff; ff.
+  Qed.
+
+  Theorem get_multi_step_reverse_spec : forall n E s,
+    List.length (all_in_rel E) - List.length s <= n ->
+    forall c c',
+    In c' (get_multi_step_reverse' c E s) <->
+    (In c' (get_all_one_step_reverse E c) \/
+     (exists c'', In c'' (get_all_one_step_reverse E c) /\
+                  In c' (get_multi_step_reverse' c'' E (set_add dec_eq c s)))).
+  Proof.
+  Admitted.
+
+
+
+  Lemma get_multi_step_reverse_trans : forall n c c' E s,
+    List.length (all_in_rel E) - List.length s <= n ->
     In c' (get_multi_step_reverse' c E s) ->
     forall c'',
       In c'' (get_multi_step_reverse' c' E s) ->
       In c'' (get_multi_step_reverse' c E s).
   Proof.
+    intros.
+    eapply get_multi_step_reverse_spec in H0.
+    eapply get_multi_step_reverse_spec in H1.
+    elim_all_contras; ff l.
+    - admit.
+    - admit.
+    - 
+    find_eapply_lem_hyp get_multi_step_reverse_spec; ff l.
+    find_eapply_lem_hyp get_multi_step_reverse_spec.
+    elim_all_contras; ff l.
+    - admit.
+    - pp (get_multi_step_reverse_spec _ _ _ H).
+    ff.
+
+
+    induction n; ff.
+    - ltac1:(simp get_multi_step_reverse' in *); ff l.
+    - ltac1:(simp get_multi_step_reverse' in *); ff l;
+      erewrite set_in_fold_left_union in *; ff l.
+      elim_all_contras; ff l.
+      * (* both in one step *)
+        destruct (in_dec dec_eq c'' (get_all_one_step_reverse E c)); ff;
+        right.
+        exists c'; split; ff.
+        eapply get_one_get_multi'; ff l.
+        erewrite set_add_iff in *; ff.
+      * (* c' in c, c'' multi-step c' *)
+        destruct (in_dec dec_eq c'' (get_all_one_step_reverse E c)); ff;
+        right.
+        unfold set_In in *.
+
+        admit.
+
+
+        destruct (dec_eq c c'), (dec_eq v c'), (dec_eq v c); ff.
+        ++ find_eapply_lem_hyp get_multi_step_self_nil; ff.
+        ++ 
+          exists c'; split; ff.
+          eapply IHn; ff l.
+          -- admit.
+          -- eapply get_one_get_multi'; ff l.
+              erewrite set_add_iff in *; ff.
+          -- admit.
+        ++ exists c'; split; ff.
+          eapply IHn; ff l.
+          -- admit.
+          -- eapply get_one_get_multi'; ff l.
+            erewrite set_add_iff in *; ff.
+          -- ff.  admit.
+      * (* c' multi-step c, c'' in c' *)
+        admit.
+      * (* both multi-step *)
+        admit.
+
+          erewrite set_in_fold_left_union in *; ff l.
+        split.
+        
+      * assert (S n0 <= 0). {
+          erewrite <- Heqn1, <- Heqn0.
+          erewrite Nat.sub_le_mono_r; ff.
+          eapply union_non_empty_len_more_r.
+        }
+        lia.
+      * elim_all_contras.
+        + left; eapply set_add_intro; ff.
+        + ff.
+          eapply IHn in H1.
+          --  
+            right.
+            exists v.
+            split; ff.
+            eapply set_add_intro; ff.
+          -- erewrite length_set_add; ff.
+            destruct (List.length (all_in_rel E)); ff l.
+      * elim_all_contras.
+        eapply IHn in H1; ff l.
+        erewrite length_set_add; ff.
+        destruct (List.length (all_in_rel E)); ff l.
+
     induction E; ff.
-    ltac1:(simp get_multi_step_reverse' in *); ff; unfold set_fold_left in *; unfold union in *; erewrite set_in_fold_left_union in *; ff.
+    ltac1:(simp get_multi_step_reverse' in *); ff; 
+    erewrite set_in_fold_left_union in *; ff.
     - destruct H; destruct H0.
       + right. exists c'. split; auto.
-        ltac1:(simp get_multi_step_reverse' in *); ff; unfold set_fold_left in *; unfold union in *; ff.
+        ltac1:(simp get_multi_step_reverse' in *); ff.
 
 
   (*
@@ -413,6 +519,42 @@ Section Sets.
   Admitted.
 
 End Sets.
+
+unfold get_multi_step_reverse.
+ltac1:(simp get_multi_step_reverse' in *); ff.
+ltac1:(simp get_multi_step_reverse' in *); ff.
+ltac1:(simp get_multi_step_reverse' in *); ff.
+ltac1:(simp get_multi_step_reverse' in *); ff.
+ltac1:(simp get_multi_step_reverse' in *); ff.
+ltac1:(simp get_multi_step_reverse' in *); ff.
+ltac1:(simp get_multi_step_reverse' in *); ff.
+ltac1:(simp get_multi_step_reverse' in *); ff.
+ltac1:(simp get_multi_step_reverse' in *); ff.
+ltac1:(simp get_multi_step_reverse' in *); ff.
+ltac1:(simp get_multi_step_reverse' in *); ff.
+ltac1:(simp get_multi_step_reverse' in *); ff.
+ltac1:(simp get_multi_step_reverse' in *); ff.
+ltac1:(simp get_multi_step_reverse' in *); ff.
+ltac1:(simp get_multi_step_reverse' in *); ff.
+ltac1:(simp get_multi_step_reverse' in *); ff.
+ltac1:(simp get_multi_step_reverse' in *); ff.
+ltac1:(simp get_multi_step_reverse' in *); ff.
+ltac1:(simp get_multi_step_reverse' in *); ff.
+ltac1:(simp get_multi_step_reverse' in *); ff.
+ltac1:(simp get_multi_step_reverse' in *); ff.
+ltac1:(simp get_multi_step_reverse' in *); ff.
+ltac1:(simp get_multi_step_reverse' in *); ff.
+ltac1:(simp get_multi_step_reverse' in *); ff.
+ltac1:(simp get_multi_step_reverse' in *); ff.
+ltac1:(simp get_multi_step_reverse' in *); ff.
+ltac1:(simp get_multi_step_reverse' in *); ff.
+ltac1:(simp get_multi_step_reverse' in *); ff.
+ltac1:(simp get_multi_step_reverse' in *); ff.
+ltac1:(simp get_multi_step_reverse' in *); ff.
+ltac1:(simp get_multi_step_reverse' in *); ff.
+
+ff.
+
 
 Arguments get_all_one_step_reverse {A} _ _.
 Arguments get_multi_step_reverse {A} _ _.
